examples/machine-code/graph/stack_introLib.sml
@@ -42,22 +42,22 @@ local
   fun get_pc_pat () = let
     val (_,_,_,pc) = get_tools ()
     in ``^pc w`` end
-  val r13 = mk_var("r13",``:word32``)
-  fun dest_r13 q = let
-    val r13_pat = case !arch_name of
+  fun dest_sp q = let
+    val sp_pat = case !arch_name of
                     ARM => ``arm_REG (R_mode mode 13w) r13``
                   | M0 => ``m0_REG RName_SP_main r13``
-                  | RISCV => ``riscv_REG RName_SP_main r13``
-    val tm = find_term (can (match_term r13_pat)) q |> rand
+                  | RISCV => ``riscv_REG 2w r2``
+    val sp = sp_pat |> rand
+    val tm = find_term (can (match_term sp_pat)) q |> rand
     in let val (x,y) = wordsSyntax.dest_word_add tm
-           val _ = x = r13 orelse fail()
+           val _ = x = sp orelse fail()
        in y |> wordsSyntax.dest_n2w |> fst |> numSyntax.int_of_term end
        handle HOL_ERR _ =>
        let val (x,y) = wordsSyntax.dest_word_sub tm
-           val _ = x = r13 orelse fail()
+           val _ = x = sp orelse fail()
        in 0-(y |> wordsSyntax.dest_n2w |> fst |> numSyntax.int_of_term) end
        handle HOL_ERR _ =>
-       if tm = r13 then 0 else failwith "unexpected value assigned to r13" end
+       if tm = sp then 0 else failwith "unexpected value assigned to sp" end
   fun get_pc_num th = let
     val pc_pat = get_pc_pat ()
     val (_,p,_,_) = dest_spec (concl th)
@@ -66,7 +66,7 @@ local
 in
   fun STACK_INTRO_RULE stack_accesses th = let
     val (_,p,_,q) = dest_spec (concl th)
-    val (n,must_intro) = (dest_r13 q,true)
+    val (n,must_intro) = (dest_sp q,true)
       handle HOL_ERR _ => (0,mem (get_pc_num th) stack_accesses)
     in if n <> 0 orelse must_intro then STACK_MEMORY_INTRO_RULE th else th end
   handle HOL_ERR e =>
