examples/machine-code/graph/decompile_testScript.sml
@@ -17,4 +17,11 @@ val fast = false;
 val ignore_names = "";
 val res = decomp base_name fast ignore_names;
 
+(* RISC-V *)
+
+val base_name = "loop-riscv/example"
+val fast = false;
+val ignore_names = "";
+val res = decomp base_name fast ignore_names;
+
 val _ = export_theory();
